books/centaur/aignet/top.lisp
@@ -1,0 +1,536 @@
+; AIGNET - And-Inverter Graph Networks
+; Copyright (C) 2013 Centaur Technology
+;
+; Contact:
+;   Centaur Technology Formal Verification Group
+;   7600-C N. Capital of Texas Highway, Suite 300, Austin, TX 78731, USA.
+;   http://www.centtech.com/
+;
+; License: (An MIT/X11-style license)
+;
+;   Permission is hereby granted, free of charge, to any person obtaining a
+;   copy of this software and associated documentation files (the "Software"),
+;   to deal in the Software without restriction, including without limitation
+;   the rights to use, copy, modify, merge, publish, distribute, sublicense,
+;   and/or sell copies of the Software, and to permit persons to whom the
+;   Software is furnished to do so, subject to the following conditions:
+;
+;   The above copyright notice and this permission notice shall be included in
+;   all copies or substantial portions of the Software.
+;
+;   THE SOFTWARE IS PROVIDED "AS IS", WITHOUT WARRANTY OF ANY KIND, EXPRESS OR
+;   IMPLIED, INCLUDING BUT NOT LIMITED TO THE WARRANTIES OF MERCHANTABILITY,
+;   FITNESS FOR A PARTICULAR PURPOSE AND NONINFRINGEMENT. IN NO EVENT SHALL THE
+;   AUTHORS OR COPYRIGHT HOLDERS BE LIABLE FOR ANY CLAIM, DAMAGES OR OTHER
+;   LIABILITY, WHETHER IN AN ACTION OF CONTRACT, TORT OR OTHERWISE, ARISING
+;   FROM, OUT OF OR IN CONNECTION WITH THE SOFTWARE OR THE USE OR OTHER
+;   DEALINGS IN THE SOFTWARE.
+;
+; Original author: Sol Swords <sswords@centtech.com>
+
+(in-package "AIGNET")
+(include-book "aig-cnf")
+(include-book "aiger")
+(include-book "aignet-absstobj")
+(include-book "aig-sim")
+(include-book "arrays")
+(include-book "bit-lemmas")
+(include-book "cnf")
+(include-book "construction")
+(include-book "copying")
+(include-book "eval")
+(include-book "from-hons-aig-fast")
+(include-book "from-hons-aig")
+(include-book "litp")
+(include-book "portcullis")
+(include-book "prune")
+(include-book "refcounts")
+(include-book "semantics")
+(include-book "snodes")
+(include-book "to-hons-aig")
+(include-book "types")
+(include-book "vecsim")
+
+(xdoc::add-resource-directory "aignet" "images")
+
+(defxdoc aignet
+  :parents (acl2::boolean-reasoning)
+  :short "An efficient, @(see stobj)-based And-Inverter Graph (AIG)
+representation for Boolean functions and finite-state machines."
+
+  :long "<h3>Background</h3>
+
+<p>At its most basic, an AIG is a DAG whose nodes are either AND gates,
+outputs, or inputs.  Outputs have 1 descendant (fanin), ANDs have 2, and inputs
+have none.  An edge may point to an AND or an input, but not an output.  Each
+edge has a Boolean attribute signifying whether it is negated or not.  Such an
+AIG is <b>combinational</b>: it represents a stateless circuit that produces
+outputs that are Boolean functions of its inputs.</p>
+
+<p>A <b>sequential</b> AIG extends this to directly model circuits with
+internal state that responds to inputs that are changing over time.  Here the
+input and outputs to the AIG are divided into two categories, <i>register</i>
+and <i>primary</i>.  The sequential semantics for an AIG depend on an initial
+state and a series of inputs:</p>
+
+<ul>
+
+<li>Initially, assign initial values to the register output nodes.</li>
+
+<li>Every cycle:
+
+   <ul>
+    <li>copy values from register outputs to corresponding register inputs</li>
+    <li>assign values to the primary inputs</li>
+    <li>compute values of AND gates in topological order</li>
+    <li>compute values of primary outputs and register inputs.</li>
+   </ul></li>
+
+</ul>
+
+<p>A sequential AIG can be viewed as a combinational AIG by ignoring the
+distinctions between its register and primary nodes.  But confusingly:</p>
+
+<ul>
+<li><color rgb='#0000ff'>Combinational inputs</color> = primary inputs + register <b>outputs</b></li>
+<li><color rgb='#ff0000'>Combinational outputs</color> = primary outputs + register <b>inputs</b></li>
+</ul>
+
+<p>To see this visually:</p>
+
+<img src='res/aignet/combinational.png'/>
+
+<p>That is: from the perspective of the combinational logic for the current
+cycle, the register outputs (the current values in the registers) are consumed
+just like the primary inputs.  Similarly, the register inputs (the values the
+registers will become in the next cycle) are emitted just like primary
+outputs.</p>
+
+
+
+<h3>The Aignet Library</h3>
+
+<p>The Aignet library, found in @('centaur/aignet'), is intended to provide an
+<b>efficient</b> implementation of sequential AIGs.</p>
+
+<p>We represent an AIG network as an @(see abstract-stobj).  This means that
+the Common Lisp implementation and its logical story are substantially
+different.  This is true of concrete stobjs as well, where access/update
+functions are logically defined in terms of @(see nth) and @(see update-nth)
+but implemented as array accesses.  But it is especially true for Aignet!</p>
+
+<ul>
+
+<li>Logically&mdash;for reasoning about the AIG network and proving AIG
+algorithms are correct&mdash;the AIG network is viewed as just a list of
+<i>nodes</i>.  Understanding these definitions is a first step toward
+successfully using Aignet; see @(see representation).</li>
+
+<li>For execution, the AIG is actually represented with various @(see stobj)
+arrays, largely styled after the <a
+href='http://www.eecs.berkeley.edu/~alanmi/abc/'>ABC</a> package.  Since the
+implementation is kept hidden, most users can feel free to skim or entirely
+skip the details in @(see aignet-impl).</li>
+
+</ul>
+
+<p>The low-level @(see base-api) connects these logical and executable
+definitions together, and provides the most basic operations for initializing
+the network, adding nodes to it, inspecting the contents of the nodes, and so
+on.  The rest of Aignet is built on top of this API.  Generally speaking,
+accesses are implemented as constant-time, and updates as amortized
+constant-time (since there may be array resizes).</p>
+
+
+
+<p>BOZO describe the rest of the library</p>
+
+
+<h3>Comparison with Hons-AIGs</h3>
+
+<p>Our focus on efficiency makes Aignet more difficult to work with and reason
+about than the simpler <see topic='@(url aig)'>Hons-AIG library</see>.  On the
+other hand, Aignet can sometimes be much faster than Hons-AIGs.  For a good
+introduction with a more detailed comparison of Hons-AIGs and Aignet, see:</p>
+
+<ul>
+
+<li>Jared Davis and Sol Swords.  <a
+href='http://dx.doi.org/10.4204/EPTCS.114.8'>Verified AIG Algorithms in
+ACL2</a>.  ACL2 Workshop 2013.  May, 2013.  EPTCS 114.  Pages 95-110.</li>
+
+</ul>")
+
+(xdoc::order-subtopics aignet
+                       (representation base-api semantics))
+
+
+(defxdoc representation
+  :parents (aignet)
+  :short "Logical representation of the AIG network."
+
+  :long "<p>We now describe the logical view of the @('aignet') stobj.  This
+representation serves as the foundation for reasoning about AIG algorithms and
+provides the logical basis for the @(see base-api).</p>
+
+<p>Note that these definitions are used for reasoning but typically do not get
+run.  For details about the executable representation, see @(see aignet-impl)
+instead, but most users should not need to think about those details.</p>
+
+
+<h3>The AIG Network</h3>
+
+<p>Logically, @('aignet') is simply a list of @(see node)s, where a node is of one of
+five types distinguished by a particular symbol in its CAR, called its @(see
+sequential-type) or <b>stype</b>.  Depending on its stype, a node contains 0 or
+more fields that encode the and-inverter graph.  We will discuss the meanings
+of these fields later:</p>
+
+<table>
+<tr><th>    Node Kind        </th><th>    Representation              </th></tr>
+
+<tr><td>    Primary input    </td><td>    @('(:pi)')                  </td></tr>
+<tr><td>    Register         </td><td>    @('(:reg)')                 </td></tr>
+<tr><td>    AND gate         </td><td>    @('(:gate fanin0 fanin1)')  </td></tr>
+<tr><td>    Next state       </td><td>    @('(:nxst fanin regid)')    </td></tr>
+<tr><td>    Primary output   </td><td>    @('(:po fanin)')            </td></tr>
+</table>
+
+<p>There is one other stype, @(':const'), but generally no node in the list
+actually has constant type; instead, the end of the list implicitly contains a
+constant node.  Thus, the number of nodes in the aignet is @('(+ 1 (len
+aignet))').  However, we use a different function, @(see node-count), for this
+purpose so that we can feel free to use rules that would be expensive to
+generally apply to @('len').</p>
+
+<p>Logically, an @('aignet') is constructed by simply consing new nodes onto
+it.  A newly-created or cleared @('aignet') is just @('nil'), and contains only
+the implicit constant node.</p>
+
+
+<h3>Node IDs and Node Lookups</h3>
+
+<p>Access to @('aignet') nodes is primarily by ID, which is simply the number
+of nodes that were in the @('aignet') when the node was added.  The implicit
+constant node has ID 0, the first node added to an empty aignet has ID 1, and
+so on.  Thus, the ID of a node in an aignet is the length (node-count) of the
+suffix of the aignet beginning at that node.</p>
+
+<p>To look up a node by ID, we use the function @(see lookup-id), which returns
+the unique <b>suffix</b> of length ID, or the final cdr of the aignet if the ID
+is out of bounds:</p>
+
+@(def lookup-id)
+
+<p>Note that although this looks like a quadratic algorithm, it doesn't matter
+because this is never actually executed.  Real ID lookups are carried out by
+array accesses.</p>
+
+
+<h3>Node Operations, Fanins, Register IDs</h3>
+
+<p>Gate, next state, and primary output nodes have some fields:</p>
+
+<ul>
+<li>A gate has two fanins (representing the inputs to the AND gate),</li>
+<li>A primary output or next-state has one fanin (the function of the output or next-state), and</li>
+<li>A next-state also contains an ID that should point to a register node.</li>
+</ul>
+
+<p>The fanins are @(see literal)s, which combine a node ID with a negation flag
+as a single natural number: @('(+ (* 2 id) neg)'), where neg is 1 or 0.</p>
+
+<p>There are many functions for constructing and accessing the various kinds of
+nodes.  See @(see logical-node) for a reference.  Note that these node-related
+functions are not meant to be executed; they exist only for reasoning.</p>
+
+
+<h3>IO Numbers and IO Lookups</h3>
+
+<p>Input, output, and register nodes also have an IO number distinct from their
+ID.  This is their index among nodes of their type, so, e.g., the first primary
+input node added has input number 0, etc.</p>
+
+<p>The IO number of a node can be determined by @(see stype-count), which
+counts the number of nodes of some type:</p>
+
+@(def stype-count)
+
+<p>Typically @('stype-count') is called by @(see lookup-stype), which looks up
+the @('n')th input/output/register node by its IO number, by searching for the
+unique node of the given type with the given IO number:</p>
+
+@(def lookup-stype)
+
+<p>Again these functions look terribly inefficient, but are implemented as
+array accesses.</p>
+
+<p>An final type of lookup operation allows us to find the next-state node
+for a given register ID:</p>
+
+@(def lookup-reg->nxst)
+
+
+<h3>Lowest-Level API</h3>
+
+<p>The functions described above&mdash;@('node-count'), @('lookup-id'),
+@('stype-count'), @('lookup-stype') and @('lookup-reg->nxst')&mdash;and
+the other functions for operating on logical nodes, e.g., the functions
+described under @(see logical-node) and 
+
+provide the
+logical basis for reasoning about most kinds of access to the aignet.</p>
+
+<p>However, note that these functions are typically not used directly.
+Instead, see the wrappers that implement Aignet's @(see base-api).</p>")
+
+
+(defsection aignet-impl
+  :parents (representation)
+  :short "Implementation details of Aignet's representation for execution.
+Since these details are hidden, most users can safely skip this section."
+
+  :long "<p>For background see @(see aignet) and @(see representation).</p>
+
+<p>We now describe the actual implementation of the @('aignet') stobj for
+execution. Our use of @(see abstract-stobj)s means that these details are
+completely hidden from reasoning about @('aignet') and have nothing at all to
+do with the logical view of an @('aignet') as a list of logical nodes.  You
+should not need to know these details when writing new Aignet algorithms or
+when understanding existing Aignet code!</p>
+
+
+<h3>Node Array</h3>
+
+<p>The Aignet network consists mainly of an array of nodes representing a
+topologically sorted DAG.</p>
+
+<p>Each node in the graph has an ID, which is a natural number that can be used
+to look up that node in the array.  However, often our functions take arguments
+that may be a node or its negation; we encode this as a @(see literal), as
+2*ID+NEG, where NEG is 1 signifying negated or 0 signifying not negated.</p>
+
+<p>One arbitrary well-formedness condition that we impose on all Aignet
+networks is that it must have a unique constant-false node with index 0.
+Therefore, the literal 0 is constant-false (the constant-false node, not
+negated), and the literal 1 is constant-true (the constant-false node,
+negated).</p>
+
+<p>Information about each node is stored in the node array as two consecutive
+32-bit numbers, and the node ID corresponds to its position in the array.  That
+is, the two array indices of a node are 2*ID and 2*ID+1.</p>
+
+
+<h3>Node Encoding</h3>
+
+<p>The two 32-bit values contained at these locations are broken down into two
+30-bit data slots and four extra bits.  Three of the four extra bits encode the
+<b>type</b> of the node, and the last extra bit encodes the <b>phase</b> of the
+node, which is its value when all inputs/registers are 0.  The meaning of the
+30-bit data slots depends on the type of node; in some cases it stores a
+literal.</p>
+
+<p>The encoding is broken down, least-significant bits first, as follows:</p>
+
+<table>
+<tr><th>  Size  </th><th>   Contents             </th></tr>
+<tr><td>  2     </td><td>   Combinational type   </td></tr>
+<tr><td>  30    </td><td>   Data slot 0          </td></tr>
+<tr><td>  1     </td><td>   Register flag        </td></tr>
+<tr><td>  1     </td><td>   Phase                </td></tr>
+<tr><td>  30    </td><td>   Data slot 1          </td></tr>
+</table>
+
+<p>The combinational types are encoded as follows:</p>
+
+<table>
+<tr><th>  Encoding  </th><th>   Meaning          </th></tr>
+<tr><td>  0         </td><td>   Constant false   </td></tr>
+<tr><td>  1         </td><td>   And gate         </td></tr>
+<tr><td>  2         </td><td>   Input            </td></tr>
+<tr><td>  3         </td><td>   Output           </td></tr>
+</table>
+
+<p>The register flag only applies to combinational inputs/outputs; it should be
+0 for constants/gates (but should also be ignored in those cases).  Note that
+the polarity here can be very <b>confusing</b>:</p>
+
+<ul>
+<li>An input with the register flag set is a register output,</li>
+<li>An output with the register flag set is a register input.</li>
+</ul>
+
+<p>The reason for this is described in @(see aignet): the output of a register
+is an input to the combinational logic, and the input to a register is an
+output from the combinational logic.</p>
+
+<p>So there are, in total, six types of objects, encoded as follows:</p>
+
+<table>
+<tr><th>   Name             </th><th>  Combinational Type  </th><th>   Register Flag   </th></tr>
+<tr><td>   Constant         </td><td>        0             </td><td>        -          </td></tr>
+<tr><td>   And gate         </td><td>        1             </td><td>        -          </td></tr>
+<tr><td>   Primary Input    </td><td>        2             </td><td>        0          </td></tr>
+<tr><td>   Register Output  </td><td>        2             </td><td>        1          </td></tr>
+<tr><td>   Primary Output   </td><td>        3             </td><td>        0          </td></tr>
+<tr><td>   Register Input   </td><td>        3             </td><td>        1          </td></tr>
+</table>
+
+
+<h3>Restrictions and Interpretation</h3>
+
+<p>Only objects with combinational types 0, 1, and 2&mdash;constants, gates,
+and combinational inputs&mdash;may be fanins (descendants) of AND or
+combinational output objects; combinational outputs (type 3) may not.</p>
+
+<p>The meanings of the two 30-bit data slots vary based on the type:</p>
+
+<ul>
+
+<li><b>Constants</b>.  Both data 0 slots are meaningless; they should be set to
+0 and ignored.</li>
+
+<li><b>AND gates</b>.  Data 0 and 1 are literals encoding the fanins to the
+gate.  To ensure an obvious topological ordering, the ID part of each literal
+must be less than the gate ID.</li>
+
+<li><b>Combinational inputs</b>.  Data 0 is ignored and should be 0.  Fanin 1
+gives the PI or register number, sequentially assigned and unique among
+PI/registers.</li>
+
+<li><b>Primary outputs</b>.  Data 0 is the fanin (literal) of the output, whose
+ID must (for topological ordering) be less than the output node ID.  Data 1 is
+the output number.</li>
+
+<li><b>Register inputs</b>.  Data 0 is the fanin (literal) of the register,
+whose ID must (for topological ordering) be less than this node's ID.  Fanin 1
+is the ID of the corresponding register output, which must also be less than
+this node's ID.  (The register number of the RI is the register number of the
+corresponding RO.)</li>
+
+</ul>
+
+
+<h3>Register Considerations</h3>
+
+<p>Having separate register input and output objects is somewhat awkward in
+terms of saying when a network is well-formed.  In some sense, it's not
+well-formed unless every RO has a corresponding RI.  But the RIs can't be added
+until their input cones are built, and we'd like to be able to say the network
+is well-formed in some sense while it is being built.  So while an RO has no
+corresponding RI, we will say it is simply not updated: its value under
+sequential evalutation remains the same at each frame.  A separate predicate
+can check that this isn't the case, but we won't generally require this for
+guards etc.</p>
+
+<p>Furthermore, for convenience, we also allow RIs with fanin 1 set to 0.  In
+this case they are not proper RIs because they do not connect to an RO, and
+they have no register number.  They are also basically irrelevant to any
+sequential computation, because no RI gets updated with their previous
+value.</p>
+
+<p>We require that each RI object occur later (have a larger ID) than its
+corresponding RO object.  This allows a couple of conveniences:</p>
+
+<ul>
+
+<li>There is a function for adding an RO and another function for adding an RI
+which connects it to an existing RO.  If we allowed RIs to occur first, then
+we'd need an additional pair of functions, for adding an unconnected RI and for
+adding an RO connected to an RI.  Maybe we could avoid this by separately
+allowing RO/RIs to be connected, but this seems knotty in terms of
+well-formedness.</li>
+
+<li>When doing a sequential simulation or similar operation that involves
+repeated sweeps across the AIG nodes, an RO node will be reached before the
+corresponding RI's previous value is overwritten.  So we don't need an
+addtional step of copying RI to RO values between frames.</li>
+
+</ul>
+
+<p>Also, a strategy that might alleviate any inconvenience due to needing to
+add the RO before the RI: at the point of adding the RI, check whether the
+RO already exists and add it first if not.</p>
+
+
+<h3>Other Arrays</h3>
+
+<p>An Aignet network is designed to have objects added one at a time without
+later modification.  That is, new objects may be added, but existing objects
+are not changed.  The object array itself (along with its size) contains enough
+information to fully replicate the network; in this sense, all other
+information recorded is auxiliary.</p>
+
+<p>For efficient lookups, we do also keep arrays of inputs, outputs, and
+registers.</p>
+
+<p>The input and output arrays simply hold the IDs of inputs/outputs in the
+order that they were added (as described above, each input/output object
+records its input/output numbers, i.e. the index in the input/output array that
+points back to it).</p>
+
+<p>The register array is a bit more complicated, because there are typically
+two nodes (register input and register output) associated with each register.
+Each entry in the register array contains the ID of either a register input or
+output.  If it is a register input, then the register is incomplete, i.e. its
+output hasn't been added yet.  If it is a register output, then we have a
+complete register: the register array points to the register output node, which
+points to the register input node, which has the index in the register
+array.</p>
+
+
+<h3>Source Code</h3>
+
+<p>For the full details, see the source code in @('aignet-exec.lisp') or
+@('aignet-exec-thms.lisp').</p>")
+
+
+(defsection semantics
+  :parents (aignet)
+  :short "The precise combinational and sequential semantics of Aignet
+networks, and also definitions of certain kinds of AIG network equivalence."
+
+  :long "<p>The combinational semantics of aignets is given by the function
+ID-EVAL.  This takes an aignet, a node ID, and assignments to the primary
+inputs and registers, and produces the value of that ID under those
+assignments.</p>
+
+<p>The sequential semantics of aignets is given by the function LIT-EVAL-SEQ.
+This takes an aignet, a time frame number, a literal, a 2D bit array assigning
+values to the primary inputs on each frame, and an initial assignment to the
+registers.  It produces the value of that literal under those sequential
+assignments.</p>
+
+<p>The following theorem describes @('lit-eval-seq') in terms of combinational
+evaluation:</p>
+
+ @(thm lit-eval-seq-in-terms-of-lit-eval)
+
+<p>Here, @('frame-regvals') is a function that creates a register value array
+from the previous frame's sequential evaluations of the next-state nodes
+corresponding to each register.  That is, to get the value of a literal at a
+particular timeframe, first evaluate the register next-states at the previous
+timeframe, then combinationally evaluate the literal with the resulting
+register values and the current frame's input values.</p>
+
+")
+
+
+
+
+
+#||
+
+(ld
+ "top.lisp")
+
+(include-book
+ "xdoc/save" :dir :system)
+
+(defsection acl2::boolean-reasoning
+  :parents (acl2::top)
+  :short "placeholder")
+
+(xdoc::save "./my-manual" :redef-okp t :zip-p nil)
+
+||#
