books/std/stobjs/1d-arr.lisp
@@ -1,0 +1,430 @@
+; ACL2 Standard Library
+; Copyright (C) 2008-2016 Centaur Technology
+;
+; Contact:
+;   Centaur Technology Formal Verification Group
+;   7600-C N. Capital of Texas Highway, Suite 300, Austin, TX 78731, USA.
+;   http://www.centtech.com/
+;
+; License: (An MIT/X11-style license)
+;
+;   Permission is hereby granted, free of charge, to any person obtaining a
+;   copy of this software and associated documentation files (the "Software"),
+;   to deal in the Software without restriction, including without limitation
+;   the rights to use, copy, modify, merge, publish, distribute, sublicense,
+;   and/or sell copies of the Software, and to permit persons to whom the
+;   Software is furnished to do so, subject to the following conditions:
+;
+;   The above copyright notice and this permission notice shall be included in
+;   all copies or substantial portions of the Software.
+;
+;   THE SOFTWARE IS PROVIDED "AS IS", WITHOUT WARRANTY OF ANY KIND, EXPRESS OR
+;   IMPLIED, INCLUDING BUT NOT LIMITED TO THE WARRANTIES OF MERCHANTABILITY,
+;   FITNESS FOR A PARTICULAR PURPOSE AND NONINFRINGEMENT. IN NO EVENT SHALL THE
+;   AUTHORS OR COPYRIGHT HOLDERS BE LIABLE FOR ANY CLAIM, DAMAGES OR OTHER
+;   LIABILITY, WHETHER IN AN ACTION OF CONTRACT, TORT OR OTHERWISE, ARISING
+;   FROM, OUT OF OR IN CONNECTION WITH THE SOFTWARE OR THE USE OR OTHER
+;   DEALINGS IN THE SOFTWARE.
+;
+; Original author: Sol Swords <sswords@centtech.com>
+
+(in-package "STOBJS")
+(include-book "absstobjs")
+(include-book "xdoc/str" :dir :system)
+(include-book "tools/defmacfun" :dir :system)
+(include-book "tools/templates" :dir :system)
+(include-book "centaur/misc/universal-equiv" :dir :system)
+
+;; BOZO might move this somewhere more sensible.
+;; This differs from Common Lisp typep in that it's a macro, and type must be a
+;; plain type-spec (it is not evaluated).
+(defmacro typep$ (x type)
+  (declare (xargs :guard (acl2::translate-declaration-to-guard type 'var nil)))
+  (acl2::translate-declaration-to-guard type x nil))
+
+
+(defxdoc def-1d-arr
+  :parents (std/stobjs)
+  :short "Defines a @(see abstract-stobj) that logically just appears to be a
+typed list but is implemented as an array."
+
+  :long "<p>Def-1d-arr produces an @(see abstract-stobj) and associated
+@('get'), @('set'), @('resize'), and @('length') functions.  Logically the
+stobj just looks like an (optionally) typed list.  But for execution, these
+functions are stobj array operations.</p>
+
+<p>How is this any better than just using @(see defstobj) to define a new stobj
+with an array field?  With a regular @('defstobj'), the stobj is logically
+viewed as a singleton list whose @('car') holds the contents.  With
+@('def-1d-arr') this extra layer goes away: the stobj itself, rather than its
+@('car'), looks like the list of elements.</p>
+
+<p>This difference is slight, but it can help to simplify reasoning, e.g., it
+can make @(see congruence)-based reasoning via @(see equivalence) relations
+like @(see acl2::list-equiv) and @(see acl2::set-equiv) easier to apply to your
+array, and can also make it easier to use proof strategies like @(see
+equal-by-nths).</p>
+
+<h3>Example</h3>
+
+<p>The following defines a bit array named @(see acl2::bitarr).</p>
+
+@({
+    (def-1d-arr bitarr          ;; Stobj name
+      :slotname    bit          ;; Base name for accessor functions
+      :pred        bitp         ;; Element type (optional)
+      :type-decl   bit          ;; Element type-spec (optional)
+      :fix         bfix         ;; Element fixing function (optional)
+      :default-val 0            ;; Element default value (for resizing)
+      :parents (std/stobjs))    ;; XDOC parent topics
+})
+
+
+<h3>Keyword Options</h3>
+
+<dl>
+
+<dt>@(':slotname') and @(':pkg-sym')</dt>
+
+<dd>The @(':slotname') influences the names of the array get, set, length, and
+resize functions.  In the example above, using @('bit') results in functions
+named @('get-bit'), @('set-bit'), @('bits-length'), and @('resize-bits').
+Default: @('<arrname>val').</dd>
+
+<dd>The @(':pkg-sym'), if given, determines the package in which any newly
+created symbols will be interned.  It defaults to the array name.</dd>
+
+
+<dt>@(':pred')</dt>
+
+<dd>This can be used to restrict the types of elements that can be put into the
+array.  It impacts the array recognizer's definition and the guard of the array
+functions.  The default is @('nil'), meaning that there are no restrictions and
+any kind of element can be put into the array.</dd>
+
+
+<dt>@(':default-val')</dt>
+
+<dd>This gives the default array element for resizing, i.e., the
+@(':initially') argument to the underlying @(see stobj).  This is often
+necessary when you provide a restricted @(':pred'), because the default value
+needs to satisfy the predicate.</dd>
+
+
+<dt>@(':type-decl')</dt>
+
+<dd>This provides a Common Lisp @(see acl2::type-spec) declaration for the
+array element's type.  It primarily affects memory efficiency and performance.
+It must sensibly agree with the given @('pred').</dd>
+
+
+<dt>@(':fix')</dt>
+
+<dd>Optional, requires a compatible @(':pred').  This alters the logical
+definition of the getting function so that it always produces a result of the
+correct type.  For example, by using @(':fix bfix') above, @('get-bit') will be
+defined as @('(bit-fix (nth i bitarr))') instead of just a call of @(see
+nth).</dd>
+
+<dt>@(':parents'), @(':short'), @(':long')</dt>
+
+<dd>These options are as in @(see defxdoc).  Note that you typically don't need
+to give @(':short') or @(':long') descriptions because reasonable boilerplate
+documentation can be generated automatically.</dd>
+
+</dl>")
+
+
+(defconst *def-1d-arr-events*
+  '(encapsulate
+     nil
+     (local
+      (progn
+        (include-book "data-structures/list-defthms" :dir :system)
+        (in-theory (enable nth update-nth resize-list))
+        (local (in-theory (disable acl2::resize-list-when-empty)))
+
+        (:@ :fix
+         (def-universal-equiv 1d-arr-tmp-equiv
+           :equiv-terms ((equal (_fix_ acl2::x)))))
+
+        ;; (def-universal-equiv 1d-arr-tmp-list-equiv
+        ;;   :qvars (i)
+        ;;   :equiv-terms ((1d-arr-tmp-equiv (nth i x))))
+
+        ;; (defcong 1d-arr-tmp-list-equiv 1d-arr-tmp-equiv (nth i x) 2
+        ;;   :hints(("Goal" :in-theory (e/d (1d-arr-tmp-list-equiv-necc)
+        ;;                                  (1d-arr-tmp-equiv)))))
+
+        ;; (defcong 1d-arr-tmp-list-equiv 1d-arr-tmp-list-equiv (update-nth i v x) 3
+        ;;   :hints((and stable-under-simplificationp
+        ;;               `(:expand (,(car (last clause)))))))
+
+        ;; (defcong 1d-arr-tmp-equiv 1d-arr-tmp-list-equiv (update-nth i v x) 2
+        ;;   :hints((and stable-under-simplificationp
+        ;;               `(:expand (,(car (last clause)))))))
+
+        ;; (in-theory (enable 1d-arr-tmp-list-equiv))
+
+        (:@ :pred
+         (defun 1d-arr-tmp-listp (x)
+           (if (atom x)
+               (eq x nil)
+             (and (:@ :pred (_pred_ (car x)))
+                  (1d-arr-tmp-listp (cdr x)))))
+
+         (defthm _pred_-nth-of-1d-arr-tmp-listp
+           (implies (and (1d-arr-tmp-listp x)
+                         (< (nfix n) (len x)))
+                    (_pred_ (nth n x))))
+
+         (defthm 1d-arr-tmp-listp-of-update-nth
+          (implies (and (1d-arr-tmp-listp x)
+                        (_pred_ v)
+                        (<= (nfix n) (len x)))
+                   (1d-arr-tmp-listp (update-nth n v x))))
+
+         (defthm 1d-arr-tmp-listp-of-resize-list
+           (implies (and (1d-arr-tmp-listp x)
+                         (_pred_ default))
+                    (1d-arr-tmp-listp (resize-list x n default)))
+           :hints (("goal" :in-theory '(resize-list
+                                        car-cons
+                                        cdr-cons
+                                        1d-arr-tmp-listp))))
+           )))
+
+     (defstobj _arrname_$c
+       (_slotname_s$c :type (array _type-decl_
+                                   (0))
+                      :initially _default-val_
+                      :resizable t)
+       :inline t)
+
+     (local
+      (progn
+
+        (defthm _slotname_s$cp-of-update-nth
+          (implies (and (_slotname_s$cp x)
+                        (typep$ v _type-decl_)
+                        (<= (nfix n) (len x)))
+                   (_slotname_s$cp (update-nth n v x))))
+
+        (defthm _slotname_s$cp-of-resize-list
+          (implies (and (_slotname_s$cp x)
+                        (typep$ default _type-decl_))
+                   (_slotname_s$cp (resize-list x n default)))
+           :hints (("goal" :in-theory '(resize-list
+                                        car-cons
+                                        cdr-cons
+                                        _slotname_s$cp))))))
+
+     (defun _arrname_$ap (_arrname_$a)
+       (declare (xargs :guard t :verify-guards t)
+                (ignorable _arrname_$a))
+       (:@ :pred
+        (if (atom _arrname_$a)
+            (eq _arrname_$a nil)
+          (and (_pred_ (car _arrname_$a))
+               (_arrname_$ap (cdr _arrname_$a)))))
+       (:@ (not :pred)
+        (true-listp _arrname_$a)))
+
+     (:@ :pred
+      (local (defthm _arrname_$ap-rewrite-to-1d-arr-tmp-listp
+               (equal (_arrname_$ap x)
+                      (1d-arr-tmp-listp x)))))
+
+     (defun create-_arrname_$a ()
+       (declare (xargs :guard t :verify-guards t))
+       nil)
+
+     (defun _slotname_s$a-length (_arrname_$a)
+       (declare (xargs :guard (_arrname_$ap _arrname_$a)
+                       :verify-guards t))
+       (len _arrname_$a))
+
+     (defun resize-_slotname_s$a (i _arrname_$a)
+       (declare (xargs :guard (_arrname_$ap _arrname_$a)
+                       :verify-guards t))
+       (resize-list _arrname_$a i '_default-val_))
+
+     (defun _slotname_s$ai (i _arrname_$a)
+       (declare (xargs :guard (and (_arrname_$ap _arrname_$a)
+                                   (integerp i)
+                                   (<= 0 i)
+                                   (< i (_slotname_s$a-length _arrname_$a)))
+                       :verify-guards t))
+       (:@ :fix
+        ;; outer ec-call supports fixing functions with guards
+        ;; e.g. the following sort of implementation
+        ;; (mbe :logic (if (foo-p a) a 'default-val) :exec a)
+        (ec-call (_fix_ (ec-call (nth i _arrname_$a)))))
+       (:@ (not :fix)
+        (ec-call (nth i _arrname_$a))))
+
+     (defun update-_slotname_s$ai (i v _arrname_$a)
+       (declare (xargs :guard (and (_arrname_$ap _arrname_$a)
+                                   (integerp i)
+                                   (<= 0 i)
+                                   (< i (_slotname_s$a-length _arrname_$a))
+                                   (:@ :pred (_pred_ v))
+                                   (typep$ v _type-decl_))
+                       :verify-guards t))
+       (ec-call (update-nth i
+                            (:@ :fix (_fix_ v))
+                            (:@ (not :fix) v)
+                            _arrname_$a)))
+
+     (local (defun-nx _arrname_$corr (_arrname_$c _arrname_$a)
+              (equal _arrname_$a (nth 0 _arrname_$c))))
+
+     (local (in-theory (disable nth resize-list
+                                (_arrname_$corr))))
+
+     ;; (local (set-default-hints
+     ;;         '((and stable-under-simplificationp
+     ;;                (let ((lit (car (last clause))))
+     ;;                  (and (consp lit)
+     ;;                       (eq (car lit) '1d-arr-tmp-list-equiv)
+     ;;                       `(:expand (,lit))))))))
+
+     ;; (local (defthm nths-equal-by-1d-arr-tmp-list-equiv
+     ;;          (implies (and (1d-arr-tmp-list-equiv x y)
+     ;;                        (:@ :pred (1d-arr-tmp-listp x))
+     ;;                        (< (nfix i) (len x)))
+     ;;                   (equal (equal (nth i x)
+     ;;                                 (:@ :fix (_fix_ (nth i y)))
+     ;;                                 (:@ (not :fix) (nth i y)))
+     ;;                          t))
+     ;;          :hints (("goal" :use 1d-arr-tmp-list-equiv-necc
+     ;;                   :in-theory (e/d ((:@ :fix 1d-arr-tmp-equiv))
+     ;;                                   (1d-arr-tmp-list-equiv-necc
+     ;;                                    (:@ :fix
+     ;;                                     1d-arr-tmp-list-equiv-implies-1d-arr-tmp-equiv-nth-2)
+     ;;                                    (:@ (not :fix)
+     ;;                                     1d-arr-tmp-list-equiv-implies-equal-nth-2)))
+     ;;                   :do-not-induct t))))
+
+     (local (in-theory (enable acl2::nth-of-resize-list-split)))
+
+     (defabsstobj-events _arrname_
+       :concrete _arrname_$c
+       :recognizer (_arrname_p :exec _arrname_$cp :logic _arrname_$ap)
+       :creator (create-_arrname_ :exec create-_arrname_$c :logic create-_arrname_$a)
+       :corr-fn _arrname_$corr
+       :exports ((_slotname_s-length :exec _slotname_s$c-length :logic _slotname_s$a-length)
+                 (get-_slotname_ :exec _slotname_s$ci :logic _slotname_s$ai)
+                 (set-_slotname_ :exec update-_slotname_s$ci :logic update-_slotname_s$ai)
+                 (resize-_slotname_s :exec resize-_slotname_s$c :logic resize-_slotname_s$a)))
+
+     (defxdoc _arrname_
+       :parents _parents_
+       :short (or _short_
+                  (str::cat "Abstract stobj: logically this just represents a list of
+                             @(see " (xdoc::full-escape-symbol '_pred_) ")s, but it is
+                             implemented as an array."))
+       :long (or _long_
+                 "<p>This is a simple abstract stobj array, introduced by @(see
+                  stobjs::def-1d-arr).</p>"))
+
+     (defsection ext
+       :extension _arrname_
+       ;; Doing it this way, instead of putting it in the :long, lets you overwrite
+       ;; the boilerplate :long above but still get the stobj definition.
+       :long (str::cat "@(def " (xdoc::full-escape-symbol '_arrname_) ")"))
+
+     ;; Hrmn, actually it's probably better NOT to generate docs for this, because
+     ;; the user should never care about it.
+     ;;
+     ;; (defxdoc _arrname_p
+     ;;   :parents (_arrname_)
+     ;;   :short (str::cat "Recognizer for the @(see " (xdoc::full-escape-symbol '_arrname_) ") array.")
+     ;;   :long (str::cat "<p>In guard obligations you will typically get to
+     ;;                    assume this for free as a result of your
+     ;;                    @('(declare (xargs :stobjs ...))') form.  In the logic,
+     ;;                    this is just a basic list recognizer:</p>
+     ;;                    @(def " (xdoc::full-escape-symbol '_arrname_$ap) ")"))
+
+     (defxdoc _slotname_s-length
+       :parents (_arrname_)
+       :short (str::cat "Get the length of the @(see "
+                        (xdoc::full-escape-symbol '_arrname_) ") array.")
+       :long (str::cat "<p>In the execution this just gets the array length.  The
+                        logical definition is just a wrapper for @(see len):</p>"
+                        "@(def " (xdoc::full-escape-symbol '_slotname_s$a-length) ")"))
+
+     (defxdoc get-_slotname_
+       :parents (_arrname_)
+       :short (str::cat "Read the @('n')th element of the @(see "
+                        (xdoc::full-escape-symbol '_arrname_) ") array.")
+       :long (str::cat "<p>In the execution this is an array access, but the logical
+                        definition is just a thin wrapper for @(see nth):</p>
+                        @(def " (xdoc::full-escape-symbol '_slotname_s$ai) ")"))
+
+     (defxdoc set-_slotname_
+       :parents (_arrname_)
+       :short (str::cat "Modify the @('n')th element of the @(see "
+                        (xdoc::full-escape-symbol '_arrname_) ") array.")
+       :long (str::cat "<p>In the execution this is an array write, but the logical
+                        definition is just a thin wrapper for @(see update-nth):</p>
+                        @(def " (xdoc::full-escape-symbol 'update-_slotname_s$ai) ")"))
+
+     (defxdoc resize-_slotname_s
+       :parents (_arrname_)
+       :short (str::cat "Change the length of the @(see "
+                        (xdoc::full-escape-symbol '_arrname_) " array.")
+       :long (str::cat "<p>In the execution this resizes (to grow or shrink) the
+                        underlying Common Lisp array.  The logical definition is
+                        based on @(see resize-list):</p>
+                        @(def " (xdoc::full-escape-symbol 'resize-_slotname_s$a) ")"))
+     ))
+
+
+
+(deffunmac def-1d-arr (arrname
+                       &key
+                       slotname
+                       pred
+                       fix
+                       default-val
+                       pkg-sym
+                       rename
+                       (type-decl 't)
+                       parents
+                       short
+                       long)
+  (declare (xargs :mode :program))
+  (b* (((unless (and (symbolp arrname)
+                     (not (keywordp arrname))))
+        (er hard? 'def-1d-arr "Invalid array name: ~x0" arrname))
+       ((unless (implies fix pred))
+        (er hard? 'def-1d-arr "If :fix is supplied, :pred must also be"))
+       (xdoc::mksym-package-symbol (or pkg-sym arrname))
+       (slotname (or slotname (xdoc::mksym arrname 'val)))
+       (type-decl (or type-decl `(satisfies ,pred)))
+       (features (cond ((and pred fix) '(:pred :fix))
+                       (pred '(:pred))))
+       (symsubst `((_arrname_ . ,arrname)
+                   (_slotname_ . ,slotname)
+                   (_fix_ . ,fix)
+                   (_pred_ . ,pred)
+                   (_type-decl_ . ,type-decl)
+                   (_default-val_ . ,default-val)
+                   (_parents_ . ,parents)
+                   (_short_ . ,short)
+                   (_long_ . ,long)
+                   ))
+       (strsubst (acl2::tmpl-symbol-alist-to-str-alist symsubst))
+       (symsubst (if fix symsubst
+                   (cons '(1d-arr-tmp-equiv . equal) symsubst)))
+       (tmpl
+        (template-subst *def-1d-arr-events*
+                        :features features
+                        :atom-alist symsubst
+                        :str-alist strsubst
+                        :pkg-sym xdoc::mksym-package-symbol)))
+    (if rename
+        (sublis rename tmpl)
+      tmpl)))
+
