books/std/stobjs/clone.lisp
@@ -1,0 +1,333 @@
+; ACL2 Standard Library
+; Copyright (C) 2008-2016 Centaur Technology
+;
+; Contact:
+;   Centaur Technology Formal Verification Group
+;   7600-C N. Capital of Texas Highway, Suite 300, Austin, TX 78731, USA.
+;   http://www.centtech.com/
+;
+; License: (An MIT/X11-style license)
+;
+;   Permission is hereby granted, free of charge, to any person obtaining a
+;   copy of this software and associated documentation files (the "Software"),
+;   to deal in the Software without restriction, including without limitation
+;   the rights to use, copy, modify, merge, publish, distribute, sublicense,
+;   and/or sell copies of the Software, and to permit persons to whom the
+;   Software is furnished to do so, subject to the following conditions:
+;
+;   The above copyright notice and this permission notice shall be included in
+;   all copies or substantial portions of the Software.
+;
+;   THE SOFTWARE IS PROVIDED "AS IS", WITHOUT WARRANTY OF ANY KIND, EXPRESS OR
+;   IMPLIED, INCLUDING BUT NOT LIMITED TO THE WARRANTIES OF MERCHANTABILITY,
+;   FITNESS FOR A PARTICULAR PURPOSE AND NONINFRINGEMENT. IN NO EVENT SHALL THE
+;   AUTHORS OR COPYRIGHT HOLDERS BE LIABLE FOR ANY CLAIM, DAMAGES OR OTHER
+;   LIABILITY, WHETHER IN AN ACTION OF CONTRACT, TORT OR OTHERWISE, ARISING
+;   FROM, OUT OF OR IN CONNECTION WITH THE SOFTWARE OR THE USE OR OTHER
+;   DEALINGS IN THE SOFTWARE.
+;
+; Original author: Sol Swords <sswords@centtech.com>
+
+(in-package "STOBJS")
+(include-book "std/util/bstar" :dir :system)
+(include-book "tools/rulesets" :dir :system)
+(include-book "tools/templates" :dir :system)
+(program)
+
+(defxdoc defstobj-clone
+  :parents (std/stobjs)
+  :short "Create a new stobj that is @(':congruent-to') an existing (concrete
+or abstract) stobj, and can be given to functions that operate on the old
+stobj."
+
+  :long "<p>@('Defstobj-clone') lets you easily introduce a new @(see stobj)
+that is @(':congruent-to') an existing stobj.  This allows you to have two (or
+more) copies of a stobj that coexist simultaneously.</p>
+
+<h3>Basic Example</h3>
+
+<p>If you want to write an algorithm that operates on two bit arrays, you might
+clone the @(see bitarr) to get a second stobj, @('bitarr2').  A minimal way to
+do this is:</p>
+
+@({
+    (defstobj-clone bitarr2 bitarr :suffix \"2\")
+})
+
+<p>This introduces:</p>
+
+<ul>
+
+<li>A new stobj, @('bitarr2'), which is congruent to @('bitarr'), and</li>
+
+<li>New functions that are basically renamed @('bitarr') operations.  In
+particular, whereas @('bitarr') has operations like @('get-bit') and
+@('set-bit'), we'll get new functions named @('get-bit2') and
+@('set-bit2').</li>
+
+</ul>
+
+<p>Usually you can just <b>ignore</b> these new functions.  They are added only
+because of the way that ACL2 stobj definition works and, strictly speaking, are
+not really necessary for anything else because you can still use the original
+stobj's functions on the new stobj.</p>
+
+<p>Ignoring the new functions is particularly useful when you have already
+built up more complex functionality on top of a stobj.  That is, if you've
+implemented functions like @('clear-range') and @('invert-range') or similar,
+you can just use these on @('bitarr2') without reimplementing them.</p>
+
+
+<h3>Renaming Accessors</h3>
+
+<p>On the other hand, it may occasionally be useful for code clarity to rename
+the new functions in some semantically meaningful way.  For instance, if your
+cloned bit array will be used as a seen table, it may be convenient to use
+operations like ('set-seen') instead of @('set-bit').</p>
+
+<p>To support using such semantically meaningful names, @('defstobj-clone') has
+a variety of options.  Here is a contrived example that uses all of them:</p>
+
+@({
+    (defstobj-clone fancy-bitarr bitarr
+      :strsubst ((\"GET\" . \"FETCH\")     ;; Substring replacements to make
+                 (\"SET\" . \"INSTALL\"))  ;;   (capitalized per symbol names)
+      :prefix \"MY-\"                      ;; Name prefix to add
+      :suffix \"-FOR-JUSTICE\"             ;; Name suffix to add
+      :pkg acl2::rewrite                   ;; Package for new symbols
+                                           ;;   default: new stobj name
+      )
+})
+
+<p>The result is to define new analogues of the @('bitarr') functions with the
+following names:</p>
+
+@({
+      bitarrp       -->  fancy-bitarrp
+      create-bitarr -->  create-fancy-bitarr
+      bits-length   -->  my-bits-length-for-justice
+      get-bit       -->  my-fetch-bit-for-justice
+      set-bit       -->  my-install-bit-for-justice
+      resize-bits   -->  my-resize-bits-for-justice
+})
+
+
+<h3>Alternate Syntax for Abstract Stobjs</h3>
+
+<p>For an abstract stobj, the accessors/updaters are known as \"exports\".
+Another way to specifying their names in the new stobj is to provide the
+@(':exports') argument, which should be a list of symbols corresponding to the
+exported functions from the original abstract stobj.  When this is provided,
+the other keyword arguments are unused.  For example:</p>
+
+@({
+    (defstobj-clone xx-bitarr bitarr
+      :exports (xx-size xx-nth !xx-nth xx-resize))
+})
+
+<p>Defines a new @('xx-bitarr') stobj with:</p>
+
+@({
+    bitarrp       --> xx-bitarrp
+    create-bitarr --> create-xx-bitarr
+    bits-length   --> xx-size
+    get-bit       --> xx-nth
+    set-bit       --> !xx-nth
+    resize-bits   --> xx-resize
+})")
+
+
+(defun clone-stobj-change-symbol (sym renaming)
+  (if renaming
+      (b* (((list prefix suffix strsubst pkg) renaming)
+           ((mv sub pkg?) (acl2::tmpl-str-sublis strsubst (symbol-name sym))))
+        (intern-in-package-of-symbol
+         (concatenate 'string prefix sub suffix)
+         (or pkg? pkg)))
+    sym))
+
+(defun clone-stobj-process-rename-alist (rename-alist renaming)
+  (if (atom rename-alist)
+      nil
+    (cons (cons (clone-stobj-change-symbol (caar rename-alist) renaming)
+                (clone-stobj-change-symbol (cdar rename-alist) renaming))
+          (clone-stobj-process-rename-alist (cdr rename-alist) renaming))))
+
+(defun clone-stobj-process-fields (fields renaming)
+  (if (atom fields)
+      nil
+    (cons (if (consp (car fields))
+              (cons (clone-stobj-change-symbol (caar fields) renaming)
+                    (cdar fields))
+            (clone-stobj-change-symbol (car fields) renaming))
+          (clone-stobj-process-fields (cdr fields) renaming))))
+
+
+
+
+(defun keep-nonbool-symbols (x)
+  (if (atom x)
+      nil
+    (let* ((k (car x)))
+      (if (and k (not (eq k t)) (symbolp k))
+          (cons k (keep-nonbool-symbols (cdr x)))
+        (keep-nonbool-symbols (cdr x))))))
+
+;; each field is: (fieldp type initial-val others)
+;; and others are all either function names, NIL when the functions aren't
+;; applicable, and a resizable flag (boolean).
+(defun stobj-field-template-fnnames (field-templates)
+  (if (atom field-templates)
+      nil
+    (cons (caar field-templates)
+          (append
+           (keep-nonbool-symbols (cdddar field-templates))
+           (stobj-field-template-fnnames (cdr field-templates))))))
+
+(defun stobj-template-fnnames (template)
+  (list* (car template)  ;; stobjp
+         (cadr template) ;; create-stobj
+         ;; field fns
+         (stobj-field-template-fnnames (caddr template))))
+
+
+(defun clone-stobj-process-args (stobjname args renaming)
+  (b* (((mv erp field-descriptors key-alist)
+        (acl2::partition-rest-and-keyword-args args acl2::*defstobj-keywords*))
+       ((when erp)
+        (er hard? 'defstobj-clone
+            "The stobj to be cloned had bad keyword args~%"))
+       (rename-alist (cdr (assoc-eq :renaming key-alist)))
+       (new-renaming (clone-stobj-process-rename-alist rename-alist renaming))
+       (inline (assoc-eq :inline key-alist))
+       (fields (clone-stobj-process-fields field-descriptors renaming)))
+    (append fields
+            (and renaming (list :renaming new-renaming))
+            (and inline (list :inline (cdr inline)))
+            (list
+; Matt K. mod: :doc is no longer supported for defstobj after v7-1
+             ;; :doc
+             ;; (concatenate 'string "Clone of stobj "
+             ;; (symbol-name stobjname))
+             :congruent-to stobjname))))
+
+(defun clone-stobj-rewrite (newfn oldfn formals)
+  (let ((thmname (intern-in-package-of-symbol
+                    (concatenate 'string (symbol-name newfn) "-IS-" (symbol-name oldfn))
+                    newfn)))
+    `((defthm ,thmname
+        (equal (,newfn . ,formals)
+               (,oldfn . ,formals))
+        :hints (("goal" :in-theory '(,newfn ,oldfn))
+                (and stable-under-simplificationp
+                     '(:in-theory (e/d** (clone-stobj-tmp-rules))))
+                (and stable-under-simplificationp
+                     '(:in-theory '(,newfn ,oldfn (:induction ,newfn))))))
+      (local (add-to-ruleset! clone-stobj-tmp-rules ,thmname)))))
+
+;; new and old are the lists of axiomatic defs
+(defun clone-stobj-rewrites (new old)
+  (b* (((when (atom new)) nil)
+       (newfn (caar new))
+       (formals (cadar new))
+       (oldfn (caar old)))
+    (append (clone-stobj-rewrite newfn oldfn formals)
+            (clone-stobj-rewrites (cdr new) (cdr old)))))
+
+
+
+
+
+(defun clone-base-stobj-fn (stobjname name renaming wrld)
+  (b* ((ev-wrld (acl2::decode-logical-name stobjname wrld))
+       ((when (null ev-wrld))
+        (er hard? 'defstobj-clone
+            "Unrecognized stobjname: ~x0~%" stobjname))
+       (event (acl2::access-event-tuple-form (cddar ev-wrld)))
+       ((when (not (eq (car event) 'acl2::defstobj)))
+        (er hard? 'defstobj-clone
+            "The event named ~x0 is not a defstobj event~%" stobjname))
+       ((list* & ;; defstobj
+               & ;; stobjname
+               args) event)
+       (name (or name (clone-stobj-change-symbol stobjname renaming)))
+       (new-args (clone-stobj-process-args stobjname args renaming))
+       (old-template (acl2::defstobj-template stobjname args wrld))
+       (new-template (acl2::defstobj-template name new-args wrld))
+       (old-defs (acl2::defstobj-axiomatic-defs stobjname old-template wrld))
+       (new-defs (acl2::defstobj-axiomatic-defs name new-template wrld)))
+    (list* 'encapsulate nil `(defstobj ,name . ,new-args)
+           '(local (def-ruleset! clone-stobj-tmp-rules nil))
+           (clone-stobj-rewrites new-defs old-defs))))
+
+(defun clone-absstobj-exports (exports logic-exec renaming concrete world)
+  (b* (((when (atom exports)) nil)
+       ((cons logic exec) (car logic-exec))
+       (new-sym (clone-stobj-change-symbol (car exports) renaming))
+       (protect (acl2::unprotected-export-p concrete exec world)))
+    (cons `(,new-sym :logic ,logic :exec ,exec :protect ,protect)
+          (clone-absstobj-exports
+           (cdr exports) (cdr logic-exec) renaming concrete world))))
+
+(defun clone-absstobj-fn (stobjname name renaming user-exports world)
+  (b* ((abs-info (fgetprop stobjname 'acl2::absstobj-info nil world))
+       (stobj-info (fgetprop stobjname 'acl2::stobj nil world))
+       (`(,concrete
+          (,recog-logic . ,recog-exec)
+          (,create-logic . ,create-exec)
+          . ,export-logic-exec)
+        abs-info)
+       (`(,& ,?pred ,?create . ,exports) stobj-info)
+       (exports (or user-exports exports))
+       (creator (acl2::defstobj-fnname name :creator :top nil))
+       (recognizer (acl2::defstobj-fnname name :recognizer :top nil)))
+    `(defabsstobj ,name
+       :concrete ,concrete
+       :recognizer (,recognizer :logic ,recog-logic :exec ,recog-exec)
+       :creator (,creator :logic ,create-logic :exec ,create-exec)
+       :exports ,(clone-absstobj-exports exports export-logic-exec renaming
+                                         ;; needed for computing :protect args
+                                         concrete world)
+       :congruent-to ,stobjname)))
+
+
+
+(defun clone-stobj-fn (stobjname name prefix suffix strsubst pkg exports world)
+  (declare (xargs :guard (and (stringp prefix)
+                              (stringp suffix)
+                              (alistp strsubst)
+                              (string-listp (strip-cars strsubst))
+                              (string-listp (strip-cdrs strsubst))
+                              (symbol-listp exports)
+                              (not (and (equal prefix "")
+                                        (equal suffix "")
+                                        (not strsubst)
+                                        (not exports))))))
+  (b* ((stobjp (fgetprop stobjname 'acl2::stobj nil world))
+       (absstobjp (fgetprop stobjname 'acl2::absstobj-info nil world))
+       (pkg (or pkg name))
+       ;; don't rename if exports are provided
+       (renaming (and (not exports)
+                      (list prefix suffix strsubst pkg)))
+       ((unless stobjp)
+        (er hard? 'defstobj-clone
+            "~x0 is not a stobj~%" stobjname)))
+    (if absstobjp
+        (clone-absstobj-fn stobjname name renaming exports world)
+      (if exports
+          (er hard? 'defstobj-clone
+              ":Exports is not supported for concrete stobjs")
+        (clone-base-stobj-fn stobjname name renaming world)))))
+
+
+
+(defmacro defstobj-clone (newname origname &key
+                                  strsubst
+                                  (prefix '"")
+                                  (suffix '"")
+                                  pkg
+                                  exports)
+  `(make-event (clone-stobj-fn ',origname ',newname ',prefix ',suffix
+                               ',strsubst ',pkg ',exports (w state))))
+
+
